

General Frameworks for Conditional Two-Sample Testing

Yonsei University

July 8, 2025

1 Block-wise MMD Framework

In this section, we provide a detailed account of our second framework, which is based on the block-wise MMD introduced by [Zaremba et al. \(2013\)](#). This statistic converges to a Gaussian distribution asymptotically and, with a suitably chosen block size B , can achieve higher power compared to linear-time alternatives. Throughout, we consider balanced samples with $n_1 = n_2 = 2n$ and divide the data into two equal parts:

$$\begin{aligned} D_a &:= \{V_i^{(1)}\}_{i=1}^n \cup \{V_i^{(2)}\}_{i=1}^n, \\ D_b &:= \{V_i^{(1)}\}_{i=n+1}^{2n} \cup \{V_i^{(2)}\}_{i=n+1}^{2n}. \end{aligned}$$

An estimator \hat{r}_X of the density ratio $r_X := f_X^{(1)}/f_X^{(2)}$ is fitted using D_b only. Let $S := \lfloor n/B \rfloor$ for the number of blocks. For $b = 1, \dots, S$ define the index set

$$I_b := \{(i, j) \in \mathbb{N}^2 : (b-1)B < i < j \leq bB\}.$$

The pairwise kernel contribution for $(i, j) \in I_b$ is

$$\begin{aligned} \hat{H}_{ij} &:= k(V_i^{(1)}, V_j^{(1)}) + \hat{r}_X(X_i^{(2)}) \hat{r}_X(X_j^{(2)}) k(V_i^{(2)}, V_j^{(2)}) \\ &\quad - \hat{r}_X(X_i^{(2)}) k(V_i^{(2)}, V_j^{(1)}) - \hat{r}_X(X_j^{(2)}) k(V_i^{(1)}, V_j^{(2)}). \end{aligned}$$

Let $b = 1, \dots, S$. The corresponding block statistics and their overall average are defined as follows:

$$\hat{\eta}_b := \binom{B}{2}^{-1} \sum_{(i,j) \in I_b} \hat{H}_{ij}.$$

Letting $\bar{\eta} := \frac{1}{S} \sum_{b=1}^S \hat{\eta}_b$ and $\hat{\sigma}_B^2 := \frac{1}{S-1} \sum_{b=1}^S (\hat{\eta}_b - \bar{\eta})^2$, and the studentized block-wise MMD statistic is given as

$$\widehat{\text{MMD}}_B^2 := \frac{\sqrt{S} \bar{\eta}}{\hat{\sigma}_B}.$$

To establish the asymptotic normality of $\widehat{\text{MMD}}_B^2$, we make the following assumptions. Let H_{ij} denote the quantity defined similarly to \hat{H}_{ij} , except that \hat{r}_X is replaced by the population counterpart r_X . Moreover, denote η_b as the counterpart of $\hat{\eta}_b$ using H_{ij} .

Assumption 1. Consider a class of null distributions \mathcal{P}_0 and assume that

- (a) There exist constants $c, C > 0$ such that $\inf_{P \in \mathcal{P}_0} \mathbb{E}_P[\eta_1^2] \geq c$ and $\sup_{P \in \mathcal{P}_0} \mathbb{E}_P[\eta_1^{2+\delta}] \leq C$ for some $\delta > 0$.
- (b) $\sup_{P \in \mathcal{P}_0} \mathbb{E}_P[r_X(X^{(2)})^2] < \infty$ and $\sup_{P \in \mathcal{P}_0} \mathbb{E}_P[\{\hat{r}_X(X^{(2)}) - r_X(X^{(2)})\}^2] = o(n^{-1/2})$.

- (c) The kernel is uniformly bounded as $\|k\|_\infty \leq K$.
- (d) The block size B satisfies $B = o(n^\gamma)$ for some $0 < \gamma < 1$.

Assumption 1(a) specifies a moment condition for the population counterpart η_b . This condition is critical for applying the uniform central limit theorem to the block-wise statistics. Assumption 1(b) ensures that the difference between the test statistic using the estimated kernel entries $\{\hat{H}_{ij}\}_{(i,j) \in I}$ and the one using the population counterparts $\{H_{ij}\}_{(i,j) \in I}$ (where $I := \{(i,j) \in [n]^2 \mid i \neq j\}$) becomes asymptotically negligible. While this assumption is similar to one discussed by Hu and Lei (2024), it imposes a considerably weaker convergence rate requirement. Assumption 1(c) requires the kernel k to be uniformly bounded, which is typically satisfied by commonly used kernels such as the Gaussian kernel. Lastly, Assumption 1(d) sets a condition on the block size B , noting that using larger blocks incorporates more samples, which helps reduce variance. However, this also leads to increased computational cost. Importantly, having at least two blocks ($S \geq 2$) is crucial for the central limit theorem to hold for the block means, ensuring that the normalized statistic converges to a Gaussian distribution.

Theorem 1. For the class of null distributions \mathcal{P}_0 satisfying 1, $\widehat{\text{MMD}}_B^2$ converges to $N(0, 1)$ as

$$\lim_{n \rightarrow \infty} \sup_{P \in \mathcal{P}_0} \sup_{t \in \mathbb{R}} \left| \mathbb{P}_P \left(\widehat{\text{MMD}}_B^2 \leq t \right) - \Phi(t) \right| = 0.$$

Proof)

Analysis of the numerator. Using the fact that a kernel can be expressed as an inner product of feature maps, $k(x, y) = \langle \psi(x), \psi(y) \rangle$, we can rewrite $\bar{\eta}$ as

$$\bar{\eta} = \frac{1}{S} \sum_{b=1}^S \binom{B}{2}^{-1} \sum_{(i,j) \in I_b} \langle \psi(V_i^{(1)}) - \hat{r}_X(X_i^{(2)})\psi(V_i^{(2)}), \psi(V_j^{(1)}) - \hat{r}_X(X_j^{(2)})\psi(V_j^{(2)}) \rangle.$$

By adding and subtracting $r_X(X_i^{(2)})\psi(V_i^{(2)})$ and $r_X(X_j^{(2)})\psi(V_j^{(2)})$, $\sqrt{S}\bar{\eta}$ can be written as the sum of the four terms given as:

$$\begin{aligned} \text{(II)} &:= \frac{1}{\sqrt{S}} \sum_{b=1}^S \binom{B}{2}^{-1} \sum_{(i,j) \in I_b} \underbrace{\langle \psi(V_i^{(1)}) - r_X(X_i^{(2)})\psi(V_i^{(2)}), \psi(V_j^{(1)}) - r_X(X_j^{(2)})\psi(V_j^{(2)}) \rangle}_{:= \eta_b} \\ \text{(III)} &:= \frac{1}{\sqrt{S}} \sum_{b=1}^S \binom{B}{2}^{-1} \sum_{(i,j) \in I_b} \underbrace{\langle \psi(V_i^{(1)}) - r_X(X_i^{(2)})\psi(V_i^{(2)}), \psi(V_j^{(2)}) \rangle \cdot \{\hat{r}_X(X_j^{(2)}) - r_X(X_j^{(2)})\}}_{:= \hat{\eta}_{b,1}} \\ \text{(III)} &:= \frac{1}{\sqrt{S}} \sum_{b=1}^S \binom{B}{2}^{-1} \sum_{(i,j) \in I_b} \underbrace{\langle \psi(V_i^{(2)}), \psi(V_j^{(1)}) - r_X(X_j^{(2)})\psi(V_j^{(2)}) \rangle \cdot \{\hat{r}_X(X_i^{(2)}) - r_X(X_i^{(2)})\}}_{:= \hat{\eta}_{b,2}} \\ \text{(IV)} &:= \frac{1}{\sqrt{S}} \sum_{b=1}^S \binom{B}{2}^{-1} \sum_{(i,j) \in I_b} \underbrace{\langle \psi(V_i^{(2)}), \psi(V_j^{(2)}) \rangle \{\hat{r}_X(X_i^{(2)}) - r_X(X_i^{(2)})\} \cdot \{\hat{r}_X(X_j^{(2)}) - r_X(X_j^{(2)})\}}_{:= \hat{\eta}_{b,3}} \end{aligned}$$

Our goal is to show that, asymptotically, $\sqrt{S}\bar{\eta} = \text{(II)} + o_{\mathcal{P}_0}(1)$ holds.

1. **Term (II).** In term (II), the population density ratio is known, implying that the sequence η_1, \dots, η_S can be treated as independent and identically distributed. Under Assumption 1(a), Lemma 18 of [Shah and Peters \(2020\)](#) ensures that

$$\sup_{P \in \mathcal{P}_0} \sup_{t \in \mathbb{R}} |\mathbb{P}_P(\sigma_P^{-1}(\mathbb{I}) \leq t) - \Phi(t)| \rightarrow 0.$$

2. **Terms (III) and (IIII).** We only analyze Term (III) by symmetry, Term (IIII) can be treated in the same manner. Let $\hat{\eta}_{b,1}(i, j)$ denote the (i, j) -th pairwise component of the block estimator $\hat{\eta}_{b,1}$, capturing the interaction between samples i and j within the b -th block. Under H_0 , we first observe that each pairwise term has zero conditional mean given the density ratio estimate data D_b :

$$\begin{aligned} \mathbb{E}[\hat{\eta}_{b,1}(i, j) | D_b] &= \mathbb{E}\left[\langle \psi(V_i^{(1)}) - r_X(X_i^{(2)}) \psi(V_i^{(2)}), \psi(V_j^{(2)}) \rangle \{\hat{r}_X(X_j^{(2)}) - r_X(X_j^{(2)})\} | D_b\right] \\ &= \{\hat{r}_X(X_j^{(2)}) - r_X(X_j^{(2)})\} \underbrace{\mathbb{E}[\langle \psi(V_i^{(1)}) - r_X(X_i^{(2)}) \psi(V_i^{(2)}), \psi(V_j^{(2)}) \rangle | D_b]}_{=0 \text{ under } H_0} \\ &= 0, \end{aligned}$$

Since $\hat{\eta}_{b,1}$ is an average of these terms and D_b is fixed within each block, we have $\mathbb{E}[\hat{\eta}_{b,1} | D_b] = 0$. Taking the expectation over D_b then gives $\mathbb{E}[\hat{\eta}_{b,1}] = \mathbb{E}_{D_b}[\mathbb{E}[\hat{\eta}_{b,1} | D_b]] = 0$, establishing the unconditional mean zero. Let $A_{ij} := \langle \psi(V_i^{(1)}) - r_X(X_i^{(2)}) \psi(V_i^{(2)}), \psi(V_j^{(2)}) \rangle$ and $B_j := \hat{r}_X(X_j^{(2)}) - r_X(X_j^{(2)})$, without loss of generality let $b = 1$,

$$\begin{aligned} \mathbb{E}[\hat{\eta}_{1,1}^2 | D_b] &= \mathbb{E}\left[\left(\frac{2}{B(B-1)} \sum_{i < j}^B A_{ij} B_j\right)^2 | D_b\right] \\ &= \frac{4}{B^2(B-1)^2} \sum_{i < j} \sum_{k < \ell} \mathbb{E}[A_{ij} B_j A_{k\ell} B_\ell | D_b] \\ &\stackrel{(i)}{=} \frac{4}{B^2(B-1)^2} \left[\sum_{i < j} \mathbb{E}[A_{ij}^2 B_j^2 | D_b] + \sum_{i < j} \sum_{\substack{\ell > i \\ \ell \neq j}} \mathbb{E}[A_{ij} B_j A_{i\ell} B_\ell | D_b] \right. \\ &\quad + \sum_{i < j} \sum_{\substack{k < j \\ k \neq i}} \mathbb{E}[A_{ij} B_j A_{kj} B_j | D_b] + \sum_{i < j} \sum_{\substack{k < i \\ k \neq j}} \mathbb{E}[A_{ij} B_j A_{ki} B_i | D_b] \\ &\quad \left. + \sum_{i < j} \sum_{\substack{\ell > j \\ \ell \neq i}} \mathbb{E}[A_{ij} B_j A_{j\ell} B_\ell | D_b] \right] \\ &= \frac{2}{B(B-1)} \mathbb{E}[A_{12}^2 B_2^2 | D_b] \\ &\quad + \frac{4(B-2)}{3B(B-1)} \left\{ \mathbb{E}[A_{12} B_2 A_{13} B_3 | D_b] + \mathbb{E}[A_{13} B_3 A_{23} B_3 | D_b] + \mathbb{E}[A_{23} B_3 A_{12} B_2 | D_b] \right\} \\ &\quad + \frac{2(B-5)}{3B(B-1)} \mathbb{E}[A_{12} B_2 A_{23} B_3 | D_b] \\ &:= T_1 + T_2 + T_3, \end{aligned}$$

where (i) separate the sum into the complete match case ($i = k, j = \ell$) and the four single-overlap cases: ($i = k, j \neq \ell$), ($i \neq k, j = \ell$), ($i = \ell, j \neq k$), and ($j = k, i \neq \ell$). All remaining terms with fully

distinct indices vanish under H_0 due to conditional independence given D_b . Therefore, only the exact match and the four overlapping cases contribute to the variance expansion.

Among these, T_1 vanishes faster than T_2 and T_3 as $B \rightarrow \infty$, so we focus on bounding the latter two terms. Using the fact that $\langle \psi(x), \psi(y) \rangle = k(x, y)$ is uniformly bounded by a constant K , and assuming for each $i \in \{1, \dots, B\}$ that

$$\sup_{P \in \mathcal{P}_0} \mathbb{E}_P \left[\{ \hat{r}_X(X_i^{(2)}) - r_X(X_i^{(2)}) \}^2 \right] = o(n^{-1/2}) \quad \text{and} \quad \sup_{P \in \mathcal{P}_0} \mathbb{E}_P \left[r_X(X_i^{(2)})^2 \right] < \infty,$$

we obtain the following bounds:

$$\begin{aligned} T_2 &\lesssim \frac{K^2}{B} \left(1 + \mathbb{E}[r_X(X_2^{(2)})] \right) \left(1 + \mathbb{E}[r_X(X_3^{(2)})] \right) \mathbb{E}[\hat{r}_X(X_2^{(2)}) - r_X(X_2^{(2)})] \mathbb{E}[\hat{r}_X(X_3^{(2)}) - r_X(X_3^{(2)})] \\ &\quad + \frac{K^2}{B} \left(1 + \mathbb{E}[r_X(X_2^{(2)})^2] \right) \mathbb{E} \left[\{ \hat{r}_X(X_3^{(2)}) - r_X(X_3^{(2)}) \}^2 \right] \\ &\stackrel{(ii)}{=} o_{\mathcal{P}_0}(B^{-1}n^{-1/2}), \end{aligned}$$

where (ii) uses Cauchy–Schwarz inequality and [Lundborg et al. \(2022, Lemma S5\)](#). Similarly,

$$\begin{aligned} T_3 &\lesssim \frac{K^2}{B} \left(1 + \mathbb{E}[r_X(X_2^{(2)})] \right) \left(1 + \mathbb{E}[r_X(X_3^{(2)})] \right) \\ &\quad \times \mathbb{E}[\hat{r}_X(X_2^{(2)}) - r_X(X_2^{(2)})] \mathbb{E}[\hat{r}_X(X_3^{(2)}) - r_X(X_3^{(2)})] \\ &= o_{\mathcal{P}_0}(B^{-1}n^{-1/2}). \end{aligned}$$

Therefore, under Assumption 1(d), the conditional variance of (III) satisfies

$$\text{Var}[(\text{III}) \mid D_b] = \frac{1}{S} \sum_{b=1}^S \text{Var}[\hat{\eta}_{b,1} \mid D_b] = o_{\mathcal{P}_0} \left(\frac{1}{Bn^{1/2}} \right) = o_{\mathcal{P}_0} \left(n^{-\frac{1+2\gamma}{2}} \right),$$

for some $0 < \gamma < 1$. Applying Chebyshev’s inequality yields $(\text{III}) = o_{\mathcal{P}_0}(1)$ and similarly $(\text{IIII}) = o_{\mathcal{P}_0}(1)$.

3. **Term (IV).** The final term (IV) is defined as

$$(\text{IV}) := \sqrt{S} \cdot \frac{1}{S} \sum_{b=1}^S \hat{\eta}_{b,3}.$$

Since the kernel k is uniformly bounded by K , we have

$$\begin{aligned} |\hat{\eta}_{b,3}| &\leq K \left| \frac{2}{B(B-1)} \sum_{(i,j) \in I_b} \{ \hat{r}_X(X_i^{(2)}) - r_X(X_i^{(2)}) \} \cdot \{ \hat{r}_X(X_j^{(2)}) - r_X(X_j^{(2)}) \} \right| \\ &\leq \frac{2K}{B(B-1)} \sum_{(i,j) \in I_b} | \hat{r}_X(X_i^{(2)}) - r_X(X_i^{(2)}) | \cdot | \hat{r}_X(X_j^{(2)}) - r_X(X_j^{(2)}) | \\ &\stackrel{(i)}{\leq} \frac{K}{B(B-1)} \left(\sum_{i=(b-1)B+1}^{bB} | \hat{r}_X(X_i^{(2)}) - r_X(X_i^{(2)}) | \right)^2 \\ &\stackrel{(ii)}{\leq} \frac{K \cdot B^2}{B(B-1)} \cdot \frac{1}{B} \sum_{i=(b-1)B+1}^{bB} \{ \hat{r}_X(X_i^{(2)}) - r_X(X_i^{(2)}) \}^2, \end{aligned}$$

where (i) uses the inequality $\sum_{i < j} |a_i| |a_j| \leq \frac{1}{2} (\sum_i |a_i|)^2$, and (ii) follows from Jensen’s inequality.

Thus, for each block b , we obtain the bound

$$|\hat{\eta}_{b,3}| \leq \frac{K \cdot B^2}{B(B-1)} \cdot \frac{1}{B} \sum_{i=(b-1)B+1}^{bB} \{\hat{r}_X(X_i^{(2)}) - r_X(X_i^{(2)})\}^2 =: \Delta_b.$$

Assuming

$$\sup_{P \in \mathcal{P}_0} \mathbb{E}_P [\{\hat{r}_X(X^{(2)}) - r_X(X^{(2)})\}^2] = o(n^{-1/2}),$$

we can apply Markov's inequality to conclude that $\Delta_b = o_{\mathcal{P}_0}(n^{-1/2})$ uniformly over b .

Since $(\mathbb{IV}) = \sqrt{S} \cdot \frac{1}{S} \sum_{b=1}^S \hat{\eta}_{b,3}$, another application of Markov's inequality yields

$$(\mathbb{IV}) = \sqrt{S} \cdot o_{\mathcal{P}_0}(n^{-1/2}) = \left\lfloor \frac{n}{B} \right\rfloor^{1/2} \cdot o_{\mathcal{P}_0}(n^{-1/2}) = o_{\mathcal{P}_0}(B^{-1/2}) = o_{\mathcal{P}_0}(n^{-\gamma/2}),$$

where the final equality holds under Assumption 1(d) and which implies $(\mathbb{IV}) = o_{\mathcal{P}_0}(1)$.

Combining the bounds for all four terms, we conclude that

$$\sup_{P \in \mathcal{P}_0} \sup_{t \in \mathbb{R}} \left| \mathbb{P}_P \left(\sqrt{S} \sigma_P^{-1} \bar{\eta} \leq t \right) - \Phi(t) \right| \rightarrow 0,$$

Consistency of the variance estimate. Denoting

$$\hat{\sigma}_P^2 := \frac{1}{S-1} \sum_{b=1}^S (\hat{\eta}_b - \bar{\eta})^2,$$

We aim to demonstrate that the ratio $\hat{\sigma}_P^2 / \sigma_P^2$ converges to one in probability, which, in turn, implies $\hat{\sigma}_P / \sigma_P = 1 + o_{\mathcal{P}_0}$ following (Lundborg et al., 2022, Lemma 7). Given that the test statistic $\widehat{\text{MMD}}_B^2$ is scale-invariant, we can assume $\sigma_P^2 = 1$ without any loss of generality. Additionally, the preceding analysis confirms that $\bar{\eta} = o_{\mathcal{P}_0}(1)$. Consequently, it suffices to show that $\frac{1}{S} \sum_{b=1}^S \hat{\eta}_b$ converges to one in probability. To establish this, note that:

$$\begin{aligned} \left| \frac{1}{S} \sum_{b=1}^S \hat{\eta}_b^2 - 1 \right| &= \left| \frac{1}{S} \sum_{b=1}^S (\eta_b + \hat{\eta}_{b,1} + \hat{\eta}_{b,2} + \hat{\eta}_{b,3})^2 - 1 \right| \\ &\leq \left| \frac{1}{S} \sum_{b=1}^S \hat{\eta}_b^2 - 1 \right| + \left| \frac{1}{S} \sum_{b=1}^S (\hat{\eta}_{b,1} + \hat{\eta}_{b,2} + \hat{\eta}_{b,3})^2 \right| + 2 \left| \frac{1}{S} \sum_{b=1}^S \eta_b (\hat{\eta}_{b,1} + \hat{\eta}_{b,2} + \hat{\eta}_{b,3}) \right| \\ &\leq \left| \frac{1}{S} \sum_{b=1}^S \hat{\eta}_b^2 - 1 \right| + \left| \frac{1}{S} \sum_{b=1}^S (\hat{\eta}_{b,1} + \hat{\eta}_{b,2} + \hat{\eta}_{b,3})^2 \right| \\ &\quad + 2 \sqrt{\frac{1}{S} \sum_{b=1}^S \eta_b^2} \sqrt{\frac{1}{S} \sum_{b=1}^S (\hat{\eta}_{b,1} + \hat{\eta}_{b,2} + \hat{\eta}_{b,3})^2}, \end{aligned}$$

where the last inequality is a consequence of the Cauchy-Schwarz inequality. Applying the law of large numbers, we see that $\frac{1}{S} \sum_{b=1}^S \eta_b^2$ converges to one in probability. Consequently, the proof reduces to establishing that $\frac{1}{S} \sum_{b=1}^S (\hat{\eta}_{b,1} + \hat{\eta}_{b,2} + \hat{\eta}_{b,3})^2 = o_{\mathcal{P}_0}(1)$. This follows from showing that

$$\frac{1}{S} \sum_{b=1}^S \hat{\eta}_{b,1} = o_{\mathcal{P}_0}(1), \quad \frac{1}{S} \sum_{b=1}^S \hat{\eta}_{b,2} = o_{\mathcal{P}_0}(1), \quad \frac{1}{S} \sum_{b=1}^S \hat{\eta}_{b,3} = o_{\mathcal{P}_0}(1).$$

These results follow from the same techniques used for (III), (IIII), and (IV), together with Markov's inequality, thereby concluding the proof.

2 Cross-fitted Extension of MMD Statistic

To further enhance sample efficiency while preserving the favorable asymptotic properties of the block-wise MMD statistic, we adopt a K -fold cross-validation strategy, similar in spirit to the approach used in linear-time MMD tests.

Let the full dataset of size $2n$ be evenly partitioned into K disjoint folds, denoted by D_1, \dots, D_K , each of size $2n/K$. For each $j \in \{1, \dots, K\}$, let $D_a := D_j$ denote the held-out block used to compute the test statistic, and let $D_b := \cup_{i=1}^K D_i \setminus D_j$ be the union of the remaining $K-1$ folds used to estimate r_X . This strategy is theoretically justified because it leverages a larger portion of the data—specifically, a $(1 - 1/K)$ fraction—for estimating the density ratio, potentially leading to more accurate and stable estimation.

We compute $\bar{\eta}_j$ and $\hat{\sigma}_j$ based on D_a and D_b , following the block-wise MMD construction. The cross-fitted statistic is then defined as

$$\dagger \widehat{\text{MMD}}_{\text{B}}^2 := \frac{1}{K} \sum_{j=1}^K \frac{\sqrt{S} \bar{\eta}_j}{\hat{\sigma}_j}.$$

The following corollary extends the central limit theorem result to the cross-fitted statistic:

Corollary 1 (Asymptotic Normality of Cross-fitted Statistic). *Under the conditions stated in Theorem 1, and for a fixed $K \geq 2$, the cross-validated test statistic satisfies:*

$$\lim_{n \rightarrow \infty} \sup_{P \in \mathcal{P}_0} \sup_{t \in \mathbb{R}} \left| \mathbb{P}_P \left(\dagger \widehat{\text{MMD}}_{\text{B}}^2 \leq t \right) - \Phi(t) \right| = 0.$$

This result justifies the use of a test that rejects H_0 whenever $\dagger \widehat{\text{MMD}}_{\text{B}}^2 > \Phi^{-1}(1 - \alpha)$ as an asymptotically level- α procedure. Moreover, since each fold contributes to both estimation and evaluation in a balanced manner, this cross-fitting strategy yields a more efficient use of the data, reducing variance while maintaining theoretical guarantees.

2.1 Proof of Corollary 1

For each $j \in \{1, \dots, K\}$, the proof of Theorem 1 establishes that $\hat{\sigma}_j / \sigma_P = 1 + o_{\mathcal{P}_0}(1)$. Therefore, by Lemma 20 of [Shah and Peters \(2020\)](#), it suffices to show the asymptotic normality of the standardized statistic

$$\frac{1}{K} \sum_{j=1}^K \frac{\sqrt{S} \bar{\eta}_j}{\sigma_P},$$

where $\bar{\eta}_j$ denotes the average of block-level statistics in fold j . Let the full dataset of size $2n$ be evenly divided into $S := \frac{2n}{B}$ disjoint blocks of size B , and assume that S is divisible by K . We assign the blocks to K disjoint subsets, denoted $\mathcal{B}_1, \dots, \mathcal{B}_K$, such that each fold j contains exactly S/K blocks, i.e., $|\mathcal{B}_j| = S/K$. Each block $b \in \{1, \dots, S\}$ consists of a set of index pairs (i, j) , denoted $I_b \subset [B] \times [B]$, and the corresponding block-level statistic is defined as

$$\eta_b := \binom{B}{2}^{-1} \sum_{(i,j) \in I_b} \left\langle \psi(V_i^{(1)}) - r_X(X_i^{(2)}) \psi(V_i^{(2)}), \psi(V_j^{(1)}) - r_X(X_j^{(2)}) \psi(V_j^{(2)}) \right\rangle.$$

Then, for each fold j , we define the block-averaged statistic as

$$\bar{\eta}_j := \frac{K}{S} \sum_{b \in \mathcal{B}_j} \eta_b.$$

Summing over all folds yields

$$\sum_{j=1}^K \bar{\eta}_j = \frac{K}{S} \sum_{j=1}^K \sum_{b \in \mathcal{B}_j} \eta_b = \frac{K}{S} \sum_{b=1}^S \eta_b + o_{\mathcal{P}_0}(S^{-1/2}),$$

where we use the fact that the collection $\{\mathcal{B}_j\}$ partitions the S blocks. Importantly, $\sum_{b \in \mathcal{B}_1} \eta_b, \dots, \sum_{b \in \mathcal{B}_K} \eta_b$ are mutually independent. Hence

$$\text{Var} \left(\frac{K}{S} \sum_{j=1}^K \sum_{b \in \mathcal{B}_j} \frac{\eta_b}{\sigma_P} \right) = \frac{K^2}{S^2} \cdot K \cdot \frac{S}{K} = \frac{K^2}{S},$$

Finally, applying the central limit theorem (Shah and Peters, 2020, Lemma 18), we obtain

$$\frac{1}{K} \sum_{j=1}^K \frac{\sqrt{S} \bar{\eta}_j}{\sigma_P} = \frac{1}{K} \sum_{j=1}^K \sum_{b \in \mathcal{B}_j} \frac{\sqrt{S} \eta_b}{\sigma_P} + o_{\mathcal{P}_0}(1),$$

converges to $N(0, 1)$ as desired.

References

- Hu, X. and Lei, J. (2024). A two-sample conditional distribution test using conformal prediction and weighted rank sum. *Journal of the American Statistical Association*, 119(546):1136–1154.
- Lundborg, A. R., Kim, I., Shah, R. D., and Samworth, R. J. (2022). The Projected Covariance Measure for assumption-lean variable significance testing. *arXiv preprint arXiv:2211.02039 (accepted to the Annals of Statistics)*.
- Shah, R. D. and Peters, J. (2020). The hardness of conditional independence testing and the generalised covariance measure. *The Annals of Statistics*, 48(3):1514–1538.
- Zaremba, W., Gretton, A., and Blaschko, M. (2013). B-test: A non-parametric, low variance kernel two-sample test. *Advances in Neural Information Processing Systems*, 26.